specs/lemmas/Spec.Hash.Incremental.Lemmas.fsti
@@ -3,9 +3,12 @@ module Spec.Hash.Incremental.Lemmas
 module S = FStar.Seq
 
 open Spec.Hash.Definitions
+open Spec.Agile.Hash
+open Spec.Hash.PadFinish
 open Spec.Hash.Incremental
 
-let hash = Spec.Agile.Hash.hash
-
-val hash_is_hash_incremental (a: hash_alg) (input: bytes { S.length input <= max_input_length a }):
-  Lemma (ensures (S.equal (hash a input) (hash_incremental a input)))
+val concatenated_hash_incremental (a:hash_alg) (inp1:bytes_blocks a) (inp2:bytes)
+  : Lemma
+    (requires Seq.length (inp1 `S.append` inp2) <= max_input_length a /\ Seq.length inp2 > 0)
+    (ensures finish a (update_last a (update_multi a (init a) inp1) (S.length inp1) inp2)
+      `S.equal` hash_incremental a (inp1 `S.append` inp2))
