specs/lemmas/Spec.Hash.Incremental.fst
@@ -2,126 +2,36 @@ module Spec.Hash.Incremental
 
 module S = FStar.Seq
 
-open Spec.Agile.Hash
 open Spec.Hash.Definitions
 open Spec.Hash.PadFinish
-open FStar.Mul
-open Lib.IntTypes
+open Spec.Hash.Lemmas
 
-#set-options "--max_fuel 0 --max_ifuel 0 --z3rlimit 300"
+friend Spec.Agile.Hash
 
-let padded_block_modulo (a:hash_alg{is_blake a}) (s1 s2:bytes) (rem:nat{rem <= block_length a}) (n:nat)
-  : Lemma (requires S.length s2 == n * block_length a /\ rem <= S.length s1)
-          (ensures Spec.Blake2.get_last_padded_block (to_blake_alg a) s1 rem `S.equal`
-                   Spec.Blake2.get_last_padded_block (to_blake_alg a) (s2 `S.append` s1) rem)
-  = let last1 = Seq.slice s1 (S.length s1 - rem) (S.length s1) in
-    let s' = s2 `S.append` s1 in
-    let last2 = Seq.slice s' (S.length s' - rem) (S.length s') in
-    assert (Seq.equal last1 last2)
+#set-options "--max_fuel 0 --max_ifuel 0 --z3rlimit 50"
 
-let small_update_last_blake
-  (a:hash_alg{is_blake a}) (h:words_state a)
-  (prevlen:nat{prevlen % block_length a = 0}) (s:bytes)
+let blake2_is_hash_incremental
+  (a:hash_alg{is_blake a}) (d:bytes{Seq.length d <= max_input_length a})
   : Lemma
-    (requires S.length s + prevlen <= max_input_length a /\ S.length s <= block_length a)
-    (ensures
-      (let last_block = Spec.Blake2.get_last_padded_block (to_blake_alg a) s (S.length s) in
-      update_last_blake a h prevlen s ==
-      (Spec.Blake2.blake2_update_block (to_blake_alg a) true (v (snd h +. u64 (S.length s))) last_block (fst h), u64 0)))
-   = let (nb, rem) = Spec.Blake2.split (to_blake_alg a) (S.length s) in
-     let blocks = Seq.slice s 0 (nb * block_length a) in
-     let h' = update_multi a h blocks in
-     Spec.Hash.Lemmas.update_multi_zero a h;
-     assert (h == h')
+    (Spec.Blake2.blake2 (to_blake_alg a) d 0 Seq.empty (Spec.Blake2.max_output (to_blake_alg a)) ==
+     hash_incremental a d)
+  = admit()
 
-let blake_split_same_modulo (a:hash_alg{is_blake a}) (len1 len2:nat) (n:nat)
-  : Lemma (requires len1 + n * block_length a = len2 /\ len1 > 0)
-          (ensures snd (Spec.Blake2.split (to_blake_alg a) len1) ==
-                   snd (Spec.Blake2.split (to_blake_alg a) len2))
-  = ()
-
-#push-options "--z3rlimit 2500"
-
-let concatenated_hash_incremental_blake (a:hash_alg{is_blake a}) (inp1:bytes_blocks a) (inp2:bytes)
-  : Lemma
-    (requires Seq.length (inp1 `S.append` inp2) <= max_input_length a /\ Seq.length inp2 > 0)
-    (ensures finish a (update_last_blake a (update_multi a (init a) inp1) (S.length inp1) inp2)
-      `S.equal` hash_incremental a (inp1 `S.append` inp2))
-  = let open FStar.Mul in
-    let h = init a in
-
-    let h1 = update_multi a h inp1 in
-    let h2 = update_last_blake a h1 (S.length inp1) inp2 in
-    let n = S.length inp2 / (block_length a) in
-    let n:nat = if S.length inp2 % block_length a = 0 && n > 0 then n-1 else n in
-    let nb, rem = Spec.Blake2.split (to_blake_alg a) (S.length inp2) in
-
-    let bs2, l2 = S.split inp2 (n * block_length a) in
-
-    assert (S.length l2 == S.length inp2 - (n * block_length a));
-    let h3 = update_multi a h1 bs2 in
-
-    let input = inp1 `S.append` inp2 in
-    let n' = S.length input / (block_length a) in
-    let n':nat = if S.length input % block_length a = 0 && n' > 0 then n'-1 else n' in
-    blake_split_same_modulo a (S.length inp2) (S.length input) (S.length inp1 / (block_length a));
-    let bs, l = S.split input (n' * (block_length a)) in
-
-    assert (l `S.equal` l2);
-    assert (bs `S.equal` (inp1 `S.append` bs2));
-
-    Spec.Hash.Lemmas.update_multi_associative a h inp1 bs2;
-    assert (h3 == update_multi a h bs);
-
-    assert (nb == n);
-
-    let h4 = update_last_blake a h3 (S.length inp1 + S.length bs2) l2 in
-
-    let last_block = Spec.Blake2.get_last_padded_block (to_blake_alg a) l2 (S.length l2) in
-    padded_block_modulo a l2 bs2 rem n;
-
-    small_update_last_blake a h3 (S.length inp1 + S.length bs2) l2
-
-
-#push-options "--z3rlimit 100"
-
-let concatenated_hash_incremental_md (a:hash_alg{is_md a}) (inp1:bytes_blocks a) (inp2:bytes)
-  : Lemma
-    (requires Seq.length (inp1 `S.append` inp2) <= max_input_length a)
-    (ensures finish a (update_last a (update_multi a (init a) inp1) (S.length inp1) inp2)
-      `S.equal` hash_incremental a (inp1 `S.append` inp2))
-  = admit();
-    allow_inversion hash_alg;
-    let len = S.length inp2 in
-    calc (S.equal) {
-    finish a (update_last a (update_multi a (init a) inp1)
-        (S.length inp1) inp2);
-    (S.equal) { }
-      finish a (update_multi a (update_multi a (init a) inp1)
-        (S.append inp2 (pad a (S.length inp1 + len))));
-    (S.equal) { }
-      finish a (update_multi a (init a)
-        (S.append inp1
-          (S.append inp2 (pad a (S.length inp1 + len)))));
-    (S.equal) { S.append_assoc
-      inp1
-      inp2
-      (pad a (S.length inp1 + len))
-    }
-      finish a (update_multi a (init a)
-        (S.append (S.append inp1 inp2)
-          (pad a (S.length inp1 + len))));
-    (==) { }
-      Spec.Agile.Hash.hash a (S.append inp1 inp2);
-    };
-    hash_is_hash_incremental a (S.append inp1 inp2)
-
-#pop-options
-
-let concatenated_hash_incremental (a:hash_alg) (inp1:bytes_blocks a) (inp2:bytes)
-  : Lemma
-    (requires Seq.length (inp1 `S.append` inp2) <= max_input_length a /\ Seq.length inp2 > 0)
-    (ensures finish a (update_last a (update_multi a (init a) inp1) (S.length inp1) inp2)
-      `S.equal` hash_incremental a (inp1 `S.append` inp2))
-   = if is_blake a then concatenated_hash_incremental_blake a inp1 inp2
-     else concatenated_hash_incremental_md a inp1 inp2
+let hash_is_hash_incremental (a: hash_alg) (input: bytes { S.length input <= max_input_length a }):
+  Lemma (ensures (S.equal (hash a input) (hash_incremental a input)))
+=
+  if is_blake a then (blake2_is_hash_incremental a input)
+  else
+  admit();
+  let open FStar.Mul in
+  let n = S.length input / block_length a in
+  let padding = pad a (S.length input) in
+  let padded_input = input `S.append` padding in
+  let blocks, rest = Lib.UpdateMulti.split_block (block_length a) padded_input n in
+  let blocks', rest' = S.split input (n * block_length a) in
+  S.lemma_eq_intro blocks blocks';
+  S.lemma_eq_intro (rest' `S.append` padding) rest;
+  Math.Lemmas.multiple_modulo_lemma n (block_length a);
+  S.lemma_eq_intro padded_input (blocks `S.append` rest);
+  update_multi_associative a (init a) blocks rest;
+  S.lemma_eq_intro (fst (update_multi a (init a) padded_input)) (fst (update_multi a (update_multi a (init a) blocks) rest))
