specs/lemmas/Spec.Hash.Incremental.fsti
@@ -49,8 +49,7 @@ let hash_incremental (a:hash_alg) (input:bytes{S.length input <= (max_input_leng
   let hash = update_last a hash (n * (block_length a)) l in
   finish a hash
 
-val concatenated_hash_incremental (a:hash_alg) (inp1:bytes_blocks a) (inp2:bytes)
-  : Lemma
-    (requires Seq.length (inp1 `S.append` inp2) <= max_input_length a /\ Seq.length inp2 > 0)
-    (ensures finish a (update_last a (update_multi a (init a) inp1) (S.length inp1) inp2)
-      `S.equal` hash_incremental a (inp1 `S.append` inp2))
+let hash = Spec.Agile.Hash.hash
+
+val hash_is_hash_incremental (a: hash_alg) (input: bytes { S.length input <= max_input_length a }):
+  Lemma (ensures (S.equal (hash a input) (hash_incremental a input)))
